theories/traverse.v
@@ -17,7 +17,7 @@ Notation len := length.
 From Stdlib Require Import Uint63.
 From Stdlib Require Import Array.PArray.
 From Stdlib Require Export ZifyNat ZifyUint63.
-From marble Require Import tactics bool int iteration loop wp array.
+From marble Require Import tactics bool int iteration loop array wp.
 From marble.logic Require Import sets relations dfs.
 From marble Require Import listz_buffer. (* TODO *)
 Implicit Type _i _j _k _n : int.
@@ -27,13 +27,6 @@ Generalizable All Variables.
 Set Universe Polymorphism.
 
 (* This file defines depth-first search algorithms. *)
-
-(* -------------------------------------------------------------------------- *)
-
-(* This constructs an inhabitant of a subset type. *)
-
-Local Notation exist x pf :=
-  (Specif.exist _ x pf).
 
 (* -------------------------------------------------------------------------- *)
 
